theories/StringRewriting/Reductions/CM2_HALT_to_SSTS01/SR2ab_facts.v
@@ -1,0 +1,28 @@
+Require Import List Relation_Operators Operators_Properties Lia.
+Import ListNotations.
+
+Require Import Undecidability.StringRewriting.Reductions.CM2_HALT_to_SSTS01.SR2ab.
+
+Require Import ssreflect.
+
+Lemma sym_eq_dec (x y: Symbol) : {x = y} + {x <> y}.
+Proof. by do 3 (decide equality). Qed.
+
+Lemma stepI {srs u v a b c d s t} : 
+  s = (u ++ a :: b :: v) -> t = (u ++ c :: d :: v) -> In ((a, b), (c, d)) srs ->
+  step srs s t.
+Proof. move=> -> ->. by constructor. Qed.
+
+Lemma multi_step_appI {srs u v s t} : multi_step srs s t -> multi_step srs (u ++ s ++ v) (u ++ t ++ v).
+Proof.
+  elim; [| move=> *; by apply: rt_refl | move=> *; apply: rt_trans; by eassumption ].
+  move=> {}s {}t [] u' v' > ?. 
+  apply /rt_step /(stepI (u := u ++ u') (v := v' ++ v)); last by eassumption.
+  all: by rewrite -?app_assoc.
+Qed.
+
+Lemma multi_step_applI {srs u s t} : multi_step srs s t -> multi_step srs (u ++ s) (u ++ t).
+Proof. move=> /multi_step_appI => /(_ u []). by rewrite ?app_nil_r. Qed.
+
+Lemma multi_step_apprI {srs v s t} : multi_step srs s t -> multi_step srs (s ++ v) (t ++ v).
+Proof. by move=> /multi_step_appI => /(_ [] v). Qed.
