theories/StringRewriting/Util/List_facts.v
@@ -1,0 +1,37 @@
+Require Import List.
+
+Require Import ssreflect.
+
+Lemma ForallE {X : Type} {P : X -> Prop} {l} : 
+  Forall P l -> if l is x :: l then P x /\ Forall P l else True.
+Proof. by case. Qed.
+
+Lemma Forall_repeatI {X : Type} {P : X -> Prop} {x n} : 
+  P x -> Forall P (repeat x n).
+Proof.
+  elim: n; first by constructor.
+  move=> ? IH ?. constructor; [done | by apply: IH].
+Qed.
+
+Lemma repeat_appP {X: Type} {x: X} {n m: nat} : 
+  repeat x n ++ repeat x m = repeat x (n+m).
+Proof. by elim: n; [| move=> ? /= ->]. Qed.
+
+Lemma In_appl {X : Type} {x: X} {l1 l2: list X} : In x l1 -> In x (l1 ++ l2).
+Proof. move=> ?. apply: in_or_app. by left. Qed.
+
+Lemma In_appr {X : Type} {x: X} {l1 l2: list X} : In x l2 -> In x (l1 ++ l2).
+Proof. move=> ?. apply: in_or_app. by right. Qed.
+
+Lemma map_firstn {X Y: Type} {f: X -> Y} {n} {l} : map f (firstn n l) = firstn n (map f l).
+Proof.
+  elim: n l; first done.
+  move=> n IH [|? ?]; first done.
+  move=> /=. congr cons. by apply: IH.
+Qed.
+
+Lemma map_skipn {X Y: Type} {f: X -> Y} {n} {l} : map f (skipn n l) = skipn n (map f l).
+Proof.
+  elim: n l; first done.
+  move=> n IH [|? ?]; [done | by apply: IH].
+Qed.
